src/NameGen.v
@@ -1,24 +1,51 @@
+Require Import Coq.Lists.List.
+Import ListNotations.
 Require Import compiler.Set.
 Require Export Coq.omega.Omega.
 
 Class NameGen(var vars st: Type){varsSet: set vars var} := mkNameGen {
+  (* Return a state which generates vars not contained in the given list.
+     We use list instead of set to guarantee that it's finite. *)
+  freshNameGenState: list var -> st;
+
+  (* Generate fresh var, and return new state *)
   genFresh: st -> (var * st);
+
+  (* Set of all vars which will be generated in the future *)
   allFreshVars: st -> vars;
+  
   genFresh_spec: forall (s s': st) (x: var),
     genFresh s = (x, s') ->
     x \in allFreshVars s /\
     ~ x \in allFreshVars s' /\
-    subset (allFreshVars s') (allFreshVars s)
+    subset (allFreshVars s') (allFreshVars s);
   (* could also say
      allFreshVars s' = diff (allFreshVars s) (singleton_set x)
      but that's unnecessarily strong and requires set equality *)
+
+  freshNameGenState_spec: forall l v, In v l -> ~ v \in (allFreshVars (freshNameGenState l));
 }.
 
+Definition listmax(l: list nat): nat := fold_right max 0 l.
+
+Lemma listmax_spec: forall l v, In v l -> v <= listmax l.
+Proof.
+  induction l; intros.
+  - simpl in H. contradiction.
+  - simpl in *. destruct H.
+    + subst. apply Nat.le_max_l. 
+    + pose proof (Nat.le_max_r a (listmax l)).
+      specialize (IHl v H).
+      eapply Nat.le_trans; eassumption.
+Qed.
+
 Instance NatNameGen: NameGen nat (nat -> Prop) nat := {|
+  freshNameGenState := fun l => S (listmax l);
   genFresh := fun s => (s, S s);
   allFreshVars := fun s => fun x => s <= x
 |}.
   abstract (intros; inversion H; subst; unfold subset; simpl; intuition omega).
+  abstract (unfold contains, Function_Set; intros; apply listmax_spec in H; omega).
 Defined.
-(* We use "abstract" to make genFresh_spec opaque, but "Defined" to make sure that
+(* We use "abstract" to make the proofs opaque, but "Defined" to make sure that
    "genFresh" and "allFreshVars" are transparent for reduction. *)
